src/sys_verif/notes/goose.v
@@ -296,7 +296,7 @@ func Add(a uint64, b uint64) uint64 {
 
 You will see `is_pkg_init <pkg>` in all preconditions for functions and methods. This asserts that the package (`functional` in this case) for the relevant function has been initialized. We need this precondition because initialization is where the code for `functional.Add` (the `Addⁱᵐᵖˡ` expression) is stored in a global variable where it is accessed by `func_call`. `wp_start` knows how to handle `is_pkg_init` and automatically puts it in the right place, so you don't mention it in the intro pattern passed to `wp_start`.
 
-We finish the proof with `wp_finish`. This is just a shorthand for `iApply "HΦ"` followed by some tactics to solve any trivial postcondition. Recall where `HΦ` comes from: all of our specifications are stated in continuation-passing style in the form `∀ Φ, P -∗ (Q -∗ Φ) -∗ wp e Φ`; `HΦ` is that second premise `Q -∗ Φ`.
+We finish the proof with `wp_end`. This is just a shorthand for `iApply "HΦ"` followed by some tactics to solve any trivial postcondition. Recall where `HΦ` comes from: all of our specifications are stated in continuation-passing style in the form `∀ Φ, P -∗ (Q -∗ Φ) -∗ wp e Φ`; `HΦ` is that second premise `Q -∗ Φ`.
 
 |*)
 
@@ -307,7 +307,7 @@ Lemma wp_Add (n m: w64) :
 Proof.
   wp_start as "%Hoverflow".
   wp_auto.
-  wp_finish. (* could do [iApply "HΦ". word.] *)
+  wp_end. (* could do [iApply "HΦ". word.] *)
 Qed.
 
 End goose.
