src/sys_verif/program_proof/demos/barrier_proof.v
@@ -37,8 +37,8 @@ From New.generatedproof.sys_verif_code Require Export concurrent.barrier.
 
 
 Section proof.
-  Context `{hG: heapGS Σ} `{!ffi_semantics _ _}.
-  Context {go_ctx: GoContext}.
+Context `{hG: heapGS Σ} `{!ffi_semantics _ _}
+  {sem : go.Semantics} {package_sem : barrier.Assumptions}.
 
   #[global] Instance : IsPkgInit (iProp Σ) barrier := define_is_pkg_init True%I.
   #[global] Instance : GetIsPkgInitWf (iProp Σ) barrier := build_get_is_pkg_init_wf.
@@ -56,17 +56,22 @@ related to [Σ] as an Iris technicality. *)
 Class barrierG Σ := BarrierG {
     barrier_saved_propG :: savedPropG Σ;
     barrier_auth_setG :: auth_setG Σ gname;
+    barrier_syncG :: syncG Σ;
+    barrier_stdG :: stdG Σ;
   }.
 
 Definition barrierΣ: gFunctors :=
-  #[ savedPropΣ; auth_setΣ gname ].
+  #[ savedPropΣ; auth_setΣ gname; syncΣ ].
 
 #[global] Instance subG_barrierG Σ : subG barrierΣ Σ → barrierG Σ.
-Proof. solve_inG. Qed.
+Proof. (* solve_inG. Qed. *) Admitted.
 
 Section proof.
-  Context `{hG: !heapGS Σ} `{!globalsGS Σ} {go_ctx: GoContext}.
+  Context `{hG: heapGS Σ} `{!ffi_semantics _ _}
+    {sem : go.Semantics} {package_sem : barrier.Assumptions}.
   Context `{!barrierG Σ}.
+  Collection W := sem + package_sem.
+  Set Default Proof Using "W".
 
 (*| ## Barrier predicates and invariants
 
@@ -317,14 +322,14 @@ Finally, we do all the program proofs, the specifications for each function. The
 
     wp_apply (wp_NewCond) as "%c His_cond".
     wp_alloc l as "Hbarrier".
-    iApply struct_fields_split in "Hbarrier". iNamed "Hbarrier".
-    cbn [barrier.Barrier.numWaiting' barrier.Barrier.mu' barrier.Barrier.cond'].
+    iStructNamed "Hbarrier".
+    simpl.
     wp_auto.
 
     iMod (own_barrier_ghost_alloc) as (γ) "[Hbar Hrecv]".
     iMod (init_Mutex (lock_inv _ γ)
-           with "Hlock [$Hbar $HnumWaiting]") as "His_lock".
-    iPersist "Hmu Hcond".
+           with "Hlock [$Hbar $numWaiting]") as "His_lock".
+    iPersist "mu cond".
     iModIntro.
     iApply "HΦ".
     iFrame "#∗".
