src/sys_verif/program_proof/heap_init.v
@@ -4,8 +4,9 @@ From New.generatedproof.sys_verif_code Require Export heap.
 From Perennial Require Import base.
 
 Section proof.
-Context `{hG: heapGS Σ} `{!ffi_semantics _ _}.
-Context `{!globalsGS Σ} {go_ctx: GoContext}.
+Context `{hG: heapGS Σ} `{!ffi_semantics _ _}
+  {sem : go.Semantics} {package_sem : heap.Assumptions}.
+Collection W := sem + package_sem.
 
 #[global] Instance : IsPkgInit (iProp Σ) heap := define_is_pkg_init True%I.
 #[global] Instance : GetIsPkgInitWf (iProp Σ) heap := build_get_is_pkg_init_wf.
