src/sys_verif/program_proof/prelude.v
@@ -18,17 +18,3 @@ These notations need to be distinct from the fupd notations (otherwise those
 don't parse), so they include a Unicode zero-width space after the => *)
 Notation "|={ E }=>​ Q" := (ncfupd E E Q) (only printing, at level 200, E at level 50) : bi_scope.
 Notation "|==>​ Q" := (ncfupd ⊤ ⊤ Q) (only printing, at level 200) : bi_scope.
-
-Ltac wp_finish :=
-  wp_auto;
-  repeat iModIntro;
-  first [
-      iApply "HΦ" |
-      (* if HΦ doesn't unify, maybe an equality proof is needed *)
-      iDestruct ("HΦ" with "[-]") as "HΦ"; [ | iExactEq "HΦ"; f_equal ]
-  ];
-  try solve [
-      auto;
-      iFrame;
-      word
-  ].
